---
tags:
  - physics
  - relativity
---
$$
\underline{r}'=\underline{r}-\underline{v}\cdot t
$$

And due to previous acceloration invarient all mechanical proceses are invariant under Galilean transformation.

 velocity tranformation:

$$
\underline{u}'= d \frac{\underline{r}'}{dt'}=\frac{\underline{r}'}{dt}=\frac{d}{dt}(\underline{r}-\underline{v}t)=\frac{d\underline{v}}{dt}-\underline{v}=\underline{u}-\underline{v}
$$
 
 u is respect to inertial frame while u' is to a moving frame

velocity tranformation of light:

Mi Chelson - Motley experiment

Doppler effecty

Period $=T$
frequency $=v=\frac{1}{T}$
$$\implies f'=f\left( 1+\frac{v}{v_{s}} \right)=\frac{v}{v_{s}}\underbrace{ (v+v_{s}) }{ Galilean V.T }$$
$v_{s} = \text{sound velocity}$

$$v=0\implies t_{1}=t_{2}=\frac{2l}{c}$$
$$t_{1}=\frac{l}{c-v}+\frac{l}{c+v}=\frac{2lc}{c^{2}-v^{2}}=\frac{2l}{c} \frac{1}{1-\frac{v^{^{2}}}{c^{^{2}}}}$$
$$
l^{2}+\left( \frac{vt_{2}}{2} \right)^{2}=\frac{ct_{2}}{2}^{2}\implies t_{2}=\frac{2l}{c}\frac{1}{\sqrt[  ]{ 1-\frac{v^{2}}{c^{2}} }}
$$
$$
\Delta t=t_{2}-t_{1}=\frac{2l}{c} \frac{1}{\sqrt[  ]{ 1-\frac{v^{2}}{c^{2}} }}-\frac{1}{1-\frac{v^{2}}{c^{2}}}
$$
$$
\frac{1}{1-\frac{v^{2}}{c^{2}}}\approx1+\frac{v^{2}}{c^{2}}\,,\, \frac{1}{\sqrt[  ]{ 1-\frac{v^{2}}{c^{2}} }}\approx 1+\frac{\frac{1}{2}v^{2}}{c^{2}}
$$
$$
\Delta t\approx \frac{2l}{c}\left( a+\frac{v^{2}}{c^{2}}-1-\frac{\frac{1}{2}v^{2}}{c^{2}} \right)=\frac{l}{c}\cdot \frac{v^{2}}{c^{2}}\approx \frac{1}{3}\cdot10^{-8}\sec
$$
$$
l_{opt}=c\Delta t,\,\lambda \text{ - wavelenght}
$$
$$
\delta=\frac{l_{opt}}{\lambda}=\frac{c}{\lambda}\cdot \frac{l}{c}\cdot \frac{v^{^{2}}}{c^{^{2}}}=\frac{l}{\lambda}\cdot \frac{v^{^{2}}}{c^{^{2}}}\approx 0.1
$$
$$
\delta=0 \text{ means that SoL is not effected by motion (v) of observer}
$$
Relativity principle: All laws of physics must be the same in any inertial frame.

Galilean transformation applied to EM does not provide this

###### Lorentz tf:
$$
\begin{matrix}
x'=ax-bt\,,\,ax'+bt' \\
t'=fx-gt\,,\,t= \\
\end{matrix}
$$
The O of the moving ' frame is $x'=0$ and $x=vt\implies 0=act-b\cdot t$
$x=ct$ and $x'=ct'\implies t= \frac{1}{c}(ax'+avt')=\frac{a}{c}(c+v)t'$
$t'=\frac{1}{c}(ax-avt)=\frac{a}{c}(c-v) \frac{a}{c}(c+v)t'$
$x'= \frac{x-vt}{\sqrt[  ]{ a-\frac{v^{2}}{c^{2}} }}\implies$

---

$$
\Delta s^{2}=c^{2}\Delta t^{2}-\Delta x^{2}-\Delta y^{2}-\Delta z^{2}\implies 
\Delta s^{2}+\Delta x^{2}+\Delta y^{2}+\Delta z^{2}=c^{2}\Delta t^{2}$$
$$
^{2}\implies \frac{\Delta s^{2}+\Delta x^{2}+\Delta y^{2}+\Delta z^{2}}{\Delta t^{2}}=c^{2}=\frac{\Delta s}{\Delta t}^{2}+v_{x}^{2}+v_{y}^{2}+v_{z}^{2}

$$