1ai)
$$
\frac{[M][L]^{3}}{[T]}=[M][L]^{3}[T]^{-1}
$$
1aii)
$$
\frac{[L][T]^{-1}}{[L]^{2}}=[L]^{-1}[T]^{-1}
$$
1bi)
$$
[L][T]^{-1}[M][L][T]^{-2}=[L]^{2}[M][T]^{-3} \neq\frac{[L]^{3}}{[T]}=[L]^{3}[T]^{-1}
$$
1bii)
$$
[M][L]^{-3}[T]= \frac{[M]}{[L]^{2}[L][T]^{-1}} + \frac{[M][T]}{[L]^{3}}=[M][L]^{-3}[T]
$$
1biii)
$$
[L][L][T]^{-2}=[L]^{2}[T]^{-2}=[L]^{2}[T]^{-2}+\frac{[M][L][T]^{-2}}{[M][L]^{-3}[L]^{2}}=[L]^{2}[T]^{-2}
$$
2)
$$
\dot{v}=Vi-gtj\implies \ddot{v}=-gj
$$

$$
x=Vt\qquad y=h-\frac{gt^{2}}{2}
$$