1. 
- (a) For the vectors $\mathbf{a}=(1,2,4),\mathbf{b}=(v_{1},v_{2},v_{3})$ and $\mathbf{c}=(1,2,3)$ determine 
	- (i) $\mathbf{a+b}$
$$
=(1+v_{1},2+v_{2},4+v_{3})
$$
- 
	- (ii) $\mathbf{a\cdot b}$
$$
=v_{1}+2v_{2}+4v_{3}
$$
	- (iii) $\mathbf{a\times b}$
$$
=(2v_{3}-4v_{2},4v_{1}-v_{3},v_{2}-2v_{1})
$$
	- (iv) the angle $θ$ between $\mathbf{a}$ and $\mathbf{c}$ (you may leave your answer in the form $θ = \cos ^{-1}(x)$ or $\sin ^{-1}(x)$ where $x$ is a number you have determined).
$$
\mathbf{a\cdot c=\left|a \right|\left|c \right|}\cos(x)\implies \theta=\cos ^{-1}\left(  \frac{1+4+6}{\sqrt[  ]{ 21\cdot 14 }} \right)=\cos ^{-1}\left(  \frac{11}{7\sqrt[  ]{ 6 }} \right)
$$
- (b) Let $z_{1}=\frac{\sqrt[  ]{ 2 }}{2}(1+i)$ and $z_{2}=2e^{ i3\pi/4 }$
	- (i) $z_{1}$ in modulus argument form, giving the principal value of the argument, and $z_{2}$ in the form $x + iy$
$$
z_{1}=e^{ i \frac{\pi}{4} }\qquad z_{2}=\sqrt[  ]{ 2 }(-1+i)
$$
	- (ii) $z_{1}+z_{2}$ in the form $x+iy$ 

$$
=\frac{\sqrt[  ]{ 2 }}{2}\left(1+3i \right)
$$
	- (iii) in the modulus argument form giving the principal value of the argument; and
$$

$$