[[CONICS solutions.pdf]]
[[CONICS solutions.pdf]]

1a)
$$
x^{2}+4xy-6x+4y^{2}-12y+9=0=(ax+by+c)^{2}=a^{2}x^{2} + 2abxy + b^{2}y + 2acx + 2bcy + c^{2}
$$
$$
\implies c=\pm 3\implies b=\mp 2 \implies a=\mp 1
$$
1b)
$$
x^{2} − 4xy + 2x + 4y^{2} − 4y + 1 =0=(ax+by+c)^{2}=a^{2}x^{2} + 2abxy + b^{2}y + 2acx + 2bcy + c^{2}
$$
$$
\implies c=\pm 1\implies b=\mp 2 \implies a=\pm 1
$$
2a)
$$
2x^{2} − xy + x − y^{2} + 2y − 1 = 0=(ax+by+c)^{2}=a^{2}x^{2} + 2abxy + b^{2}y + 2acx + 2bcy + c^{2}
$$
$$
c=\pm i\implies b=\mp i\implies a=\mp \frac{i}{2} \therefore
$$
$$
y=1- \frac{x}{2}
$$
2b)
$$
2x^{2} − xy + 5x − y^{2} + y + 2 = 0=(ax+by+c)^{2}=a^{2}x^{2} + 2abxy + b^{2}y + 2acx + 2bcy + c^{2}
$$
$$
c=\pm \sqrt[  ]{ 2 }\implies b=\pm \frac{1}{2\sqrt[  ]{ 2 }}\implies a=\mp \sqrt[  ]{ 2 }
$$
$$
y=4x-4
$$
3a)
$$
3x^{2} + 24x + 53 − 2y^{2} + 4y = 0 = \left( \sqrt[  ]{ 3 }x+2\sqrt[  ]{ 3 } \right) ^{2}-\left( \sqrt[  ]{ 2 }y-\sqrt[  ]{ 2 } \right) ^{2}=\frac{43}{6}= \frac{\left( x+2 \right)^{2}}{2}-\frac{(y-1)^{2}}{3}
$$
hyperbola

3b)
$$
2x^{2} − 4x + 10 + 4y^{2} + 16y = 0
$$
$$
\frac{\left(x-1 \right)^{2}}{4}+\frac{(y+2)^{2}}{2}=1
$$
Ellipse

3c)
$$
y^{2} − 2y − 11 − 6x = 0\implies \frac{\left( y-1 \right)^{2}}{6}-2=x
$$
Parabola on the y axis instead of x

4a)
$$
c=2=\sqrt[  ]{ a^{2}-b^{2} }\qquad a=3\implies b=\sqrt[  ]{ 5 }\implies \frac{x^{2}}{9}+ \frac{y^{2}}{5}=1
$$
4b)
$$
\frac{c}{a}=e\implies a=4\implies b=2\sqrt[  ]{ 3 }\implies \frac{(x-2)^{2}}{16}+\frac{(y-1)^{2}}{12}=1
$$
5a)
$$
9(x-1)^{2}+4(y+1)^{2}=36\iff \frac{(x-1)^{2}}{4}+ \frac{(y+1)^{2}}{9}=1
$$
$$
a=2,\,b=3,c=\sqrt[  ]{ 5 }
$$
Centre is $(1,-1)$ with foci being $(1,-1\pm \sqrt[  ]{ 5 })$ as this is an ellipse rotated by $90°$ about the centre with major axis as $b=3$ and minor axis as $a=2$.

5b)
$$
2(x-1)^{2}+4(y+2)^{2}=8\iff \frac{(x-1)^{2}}{4}+\frac{(y+2)^{2}}{2}=1
$$
$$
a=2,\,b=\sqrt[  ]{ 2 },\,c=\sqrt[  ]{ 2 }
$$
Centre is $(1,-2)$ with foci being $(1\pm \sqrt[  ]{ 2 },-2)$ with major axis as $a=2$ and minor axis as $b=\sqrt[  ]{ 2 }$.
