[[24_25_1RAVGLAsimexam.pdf]]

1ai) 
Where $f$ is defined on $[a,b]\setminus \{ c \}$ and $c\in(a,b)$ where as $x\to c$, $f(x)\to \ell \in \mathbb{R}$ s.t. $\forall\varepsilon>0\exists\delta>0$
$$
\left| f(x)-\ell \right| < \varepsilon \implies\left| x-c \right| < \delta
$$

1aii)
$$
\lim_{ x \to 1 } 3x+2=5
$$
$$
\left| (3x+2)-5 \right| = 3 \left| x-1 \right|  <\varepsilon
$$
$$
\left| x-1 \right| <\delta\implies \delta = \frac{\varepsilon}{3}
$$
1bi)
$$
f'(\alpha)= \lim_{ h \to 0 }  \frac{f(\alpha+h)-f(\alpha)}{h} 
$$
1bii)
$$
f'(\pi)= \lim_{ h \to 0 }  \frac{(\pi+h)^{3}-(\pi)^{3}}{h}= \lim_{ h \to 0 } \frac{3\pi^{2} h+3\pi h^{2}+h^{3}}{h}=\lim_{ h \to 0 } 3\pi^{2}+3\pi h + h^{2} \to 3\pi^{2}
$$
1ci)
Using L'Hopitals rule
$$
\lim_{ x \to 0 } \frac{\sin 7x}{\sin 4x}= \lim_{ x \to 0 } \frac{7\cos 7x}{4\cos 4x}\to\frac{7}{4}
$$
1cii)
Using AoL
$$
\lim_{ x \to \infty } \frac{6x^{2}+8x+9}{x^{2}+2x-6}=\lim_{ x \to \infty } \frac{6+\frac{8}{x}+\frac{9}{x^{2}}}{1+\frac{2}{x}-\frac{6}{x^{2}}}\to 6
$$
1di)
$$
f'(x)=(\cos x)'+(\ln x)'+(x^{4})'=4x^{3}+\frac{1}{x}-\sin x
$$
1dii)
Using quotient rule
$$
\left( \frac{\cos x-1}{e^{ x }+1} \right)'=\left( \frac{f(x)}{g(x)} \right)'= \frac{f'(x)g(x)-f(x)g'(x)}{(g(x))^{2}}= \frac{-(e^{ x }+1)\sin x-(\cos x-1)e^{ x }}{e^{ 2x }}
$$
1ei)
$$
f'(x)=6x^{2}-12x-18=0\implies x=3\text{ and } -1\therefore f'(x)<0:(-1,3)
$$
$$
f'(x)>0(x<-1)\land (x>3)
$$
1eii)
$$
f''(x)=12x-12\overset{ x=-1 }{ \underset{ x=3 }{ \implies  }} f''(-1)=-24\qquad f''(3)=24
$$
$x=3$ is a local minima and $x=-1$ is a local maxima.
2ai)
$$
a+b=(a+v_{1},2+v_{2},4+v_{3})
$$
2aii)
$$
a\cdot b=(2v_{3}-4v_{2},4v_{1}-v_{3},v_{2}-2v_{1})
$$
2aiii)
$$
a\times b= 4v_{3}
$$
$$
a\times b=|a||b|\cos \theta\implies \cos ^{-1}\left( \frac{4v_{3}}{\sqrt[  ]{ 21(v_{1}^{2}+v_{2}^{2}+v_{3}^{2}) }} \right)
$$
2bi)
$$
z_{1}= -\frac{\sqrt[  ]{ 2 }}{2}(1+i)= e^{ -i\frac{3}{4}\pi  }\qquad z_{2}=2e^{ i \frac{3}{4}\pi } = -\sqrt[  ]{ 2 }+i\sqrt[  ]{ 2 }
$$
2bii)
$$
z_{1}+z_{2}=- \frac{3\sqrt[  ]{ 2 }}{2} + i\frac{\sqrt[  ]{ 2 }}{2}
$$
2biii)
$$
z_{1}z_{2}^{-1}= e^{ -i \frac{3}{4}\pi }\left( 2e^{ i \frac{3}{4}\pi } \right)=\frac{1}{2}e^{ - i\frac{3}{2}\pi }= \frac{1}{2} e^{ i \frac{1}{2}\pi }
$$
2biv)
$$
z_{1}^{29}=e^{ -i \frac{3}{4}\pi\cdot 29 }=e^{ -i \frac{57}{4}\pi }=e^{ -i \frac{1}{4}\pi }
$$
2ci)
$$
\begin{array}{} \\
3x+2y-z&=&4 \\
2x-y+2z&=&10 \\
x-3y-4z&=&5
\end{array}

$$
$$
\begin{array}{} \\
x+3y-3z&=&-6 \\
5y+10z&=&0 \\
6y+z&=&-11
\end{array}
$$
$$
\begin{array}{} \\
x+3y-3z&=&-6 \\
5y+10z&=&0 \\
55y&=&-110
\end{array}
$$
$$
y=-2\implies z=1\implies x=3
$$
2cii)
$$
\begin{array}{} \\
3x+2y-z&=&a \\
2x-y+2z&=&0 \\
x-3y-4z&=&0
\end{array}

$$
$$
\begin{array}{} \\
x+3y-3z&=&a \\
5y+10z&=&0 \\
6y+z&=&a
\end{array}
$$
$$
\begin{array}{} \\
x+3y-3z&=&a \\
5y+10z&=&0 \\
55y&=&10a
\end{array}
$$
$$
y= \frac{2}{11}a\implies z=- \frac{1}{11}a\implies x =\frac{2}{11}a
$$