Setup:
$$
\mu_{1}=\mu_{3}=\frac{1g}{\underbrace{ 1\times SA }_{ V (volume) }},\mu_{2}=\frac{40g}{V}=4\mu_{2},A=1\times 10^{-3}, v=\lambda f
$$
$$
v^{2}=\frac{\omega^{2}}{k^{2}}=\frac{T}{\mu}\implies k_{1}=\omega \sqrt[  ]{ \frac{\mu_{1}}{T} }=k_{3}=\omega \sqrt[  ]{ \frac{\mu_{3}}{T} },k_{2}=\omega \sqrt[  ]{ \frac{\mu_{2}}{T} }
$$
1)
$$
\lambda_{1} \propto v_{1} \propto \frac{1}{k} \propto \frac{1}{\sqrt[  ]{ \mu }}\implies \lambda \propto \frac{1}{\sqrt[  ]{ \mu }}
$$
$$
\therefore \lambda_{1} \propto \frac{1}{\sqrt[  ]{ \mu_{1} }}:\lambda_{2} \propto \frac{1}{\sqrt[  ]{ \mu_{2} }}: \lambda_{3} \propto \frac{1}{\sqrt[  ]{ \mu_{3} }}
$$
$$
\lambda_{1}:\lambda_{2}:\lambda_{3}=\frac{1}{\sqrt[  ]{ \mu_{1} }}: \frac{1}{\sqrt[  ]{ 4\mu_{1} }}:\frac{1}{\sqrt[  ]{ \mu_{1} }}=1:2:1
$$
2)
$$
B_{1}= \frac{2k_{1}}{k_{1}+k_{2}}A_{1}= \frac{2\omega \sqrt[  ]{ \frac{10}{V} }}{\omega \left( \sqrt[  ]{ \frac{10}{V} }+ \sqrt[  ]{ \frac{40}{V} } \right)}A_{1}=\frac{2\sqrt[  ]{ 10 }}{\sqrt[  ]{ 10 }+\sqrt[  ]{ 40 }}A_{1}= \frac{2}{3} A_{1}=A_{2}
$$
$$
B_{2}=\frac{2k_{2}}{k_{2}+k_{1}}A_{2}= \frac{2\omega \sqrt[  ]{ \frac{40}{V} }}{\omega \left( \sqrt[  ]{ \frac{10}{V} }+ \sqrt[  ]{ \frac{40}{V} } \right)}A_{2}=\frac{4}{3}A_{2}=\frac{8}{9}A_{2}
$$
$$
\therefore \text{Amplitude of string 3 is }8.89\times 10^{-4}m
$$
