1a)
$$
P(E)=\frac{e^{ -\frac{E}{k_{B}T} }}{k_{B}T}\impl ies \int ^{\infty}_{0} \frac{e^{ -\frac{E}{k_{B}T} }}{k_{B}T} \, dE =\left[ \frac{1}{\frac{dP(E)}{dE}}\frac{e^{ -\frac{E}{k_{B}T} }}{k_{B}T} \right]^{\infty}_{0}=\left[ -k_{B}T\frac{e^{ -\frac{E}{k_{B}T} }}{k_{B}T} \right]^{\infty}_{0}=\left[ -e^{ -\frac{E}{k_{B}T} } \right]^{\infty}_{0}=0 + 1
$$

1b)
$$
uv -\int ^{}_{}u \frac{dv}{dE}  \, dE = \int ^{}_{}v\frac{du}{dE}  \, dE 
$$
$$
\frac{dv}{dE}=P(E), u= [E]^{\infty}_{0}, v= \left[ -e^{ -\frac{E}{k_{B}T} }  \right]^{\infty}_{0}, \frac{du}{dE}=1
$$
$$
[E]^{\infty}_{0}\left[ -e^{ -\frac{E}{k_{B}T} }\right]^{\infty}_{0}-\int ^{\infty}_{0} -e^{ -\frac{E}{k_{B}T} } \, dE =\left[ -Ee^{ -\frac{E}{k_{B}T} }\right]^{\infty}_{0}-\left[ k_{B}Te^{ -\frac{E}{k_{B}T} } \right]^{\infty}_{0} 
$$
$$
f'(E)=-e^{ -\frac{E}{k_{B}T} },g'(E)=\frac{1}{E},f(E)=-k_{B}Te^{ -\frac{E}{k_{B}T} },g(E)=\ln|E|
$$
$$
\lim_{ E \to \infty } \frac{f(E)}{g(E)}=\lim_{ E \to \infty } \frac{f'(E)}{g'(E)}\implies \lim_{ E \to \infty }  -Ee^{ -\frac{E}{k_{B}T} }=\lim_{ E \to \infty } \frac{-k_{B}Te^{ -\frac{E}{k_{B}T} }}{\ln E}=0
$$
$$
\therefore \int^{\infty}_{0}E\,P(E)\,dE=(0-0)-(0-k_{B}T)=k_{B}T
$$

1c)
$$
\lambda_{\mathrm{max}}=\frac{b}{T}= \frac{2.897\dots\times 10^{-3}}{2.73}=1.061\dots \times 10^{-3}m.\text{ Microwaves.}
$$

