$$
E_{tot}=m_{\pi}c^{2}+0=m_{\mu}c^{2}\gamma(v)+p_{\bar{v}}c= m_{\mu}c^{2}\gamma(v) +(m_{\mu}v\gamma(v))c=m_{\mu}\gamma(v)(c^{2}+vc)
$$
$$
=m_{\pi}c^{2}=m_{\mu}c^{2}\gamma(v)\left( 1+\frac{v}{c} \right)=m_{\mu}c^{2}\left( \frac{1+\frac{v}{c}}{\sqrt[  ]{ 1-\frac{v^{2}}{c^{2}} }} \right)
$$
$$
\implies\frac{m_{\pi}}{m_{\mu}}=  \sqrt[  ]{ \frac{1+\frac{v}{c}}{1-\frac{v}{c}} } \implies \left( \frac{m_{\pi}}{m_{\mu}} \right)^{2}= \frac{1+\frac{v}{c}}{1-\frac{v}{c}}\implies \frac{v}{c}= \frac{m_{\pi}^{2}-m_{\mu}^{2}}{m_{\pi}^{2}+m_{\mu}^{2}}
$$
$$
m_{\pi}=\frac{E_{tot}}{c^{2}},m_{\mu}= \frac{105.65MeV}{c^{2}},v=8.145\dots \times 10^{7} ms^{-1}
$$
$$
x=\gamma(v)\left( x'+ vt' \right),t'=2.2 \times 10^{-6},x'=0\implies x= \frac{v \times2.2 \times 10^{-6}+0}{\sqrt[  ]{ 1-\frac{v^{2}}{c^{2}} }}=186.19\dots m
$$